coq/Match.v
@@ -1,0 +1,123 @@
+(** * Matching and Role Homomorphisms *)
+
+Require Import String Monad Alg Role.
+Import List.ListNotations.
+Open Scope list_scope.
+(** printing <- #←# *)
+
+(** A substitution *)
+
+Definition sbst: Set := list (var * alg).
+
+Definition extend_term (ev: sbst) (v: var) (x: alg): option sbst :=
+  match lookup v ev with
+  | None => Some ((v, x) :: ev)
+  | Some y =>
+    if alg_dec x y then
+      Some ev
+    else                        (* Term clash! *)
+      None
+  end.
+
+Definition match_skey (ev: sbst) (x y: skey): option sbst :=
+  match x, y with
+  | Sv v, w => extend_term ev v (Sk w)
+  | Lt v w, Lt x y =>
+    ev <- extend_term ev v (Nm x);
+    extend_term ev w (Nm y)
+  | _, _ => None
+  end.
+
+Definition match_akey (ev: sbst) (x y: akey): option sbst :=
+  match x, y with
+  | Av v, w => extend_term ev v (Ak w)
+  | Pb v, Pb w => extend_term ev v (Nm w)
+  | Pb2 s v, Pb2 t w =>
+    if eqb s t then
+      extend_term ev v (Nm w)
+    else
+      None
+  | _, _ => None
+  end.
+
+Fixpoint match_term (ev: sbst) (x y: alg): option sbst :=
+  match x, y with
+  | Tx v, Tx w => extend_term ev v (Tx w)
+  | Dt v, Dt w => extend_term ev v (Dt w)
+  | Nm v, Nm w => extend_term ev v (Nm w)
+  | Sk v, Sk w => match_skey ev v w
+  | Ak v, Ak w => match_akey ev v w
+  | Ak (Av v), Ik w => extend_term ev v (Ik w)
+  | Ik v, Ik w => match_akey ev v w
+  | Ik (Av v), Ak w => extend_term ev v (Ik w)
+  | Ch v, Ch w => extend_term ev v (Ch w)
+  | Mg v, w => extend_term ev v w
+  | Tg s, Tg t =>
+    if eqb s t then
+      Some ev
+    else
+      None
+  | Pr v w, Pr x y =>
+    ev <- match_term ev v x;
+    match_term ev w y
+  | En v w, En x y =>
+    ev <- match_term ev v x;
+    match_term ev w y
+  | Hs v, Hs w => match_term ev v w
+  | _, _ => None
+  end.
+
+Definition match_evt (ev: sbst) (x y: evt): option sbst :=
+  match x, y with
+  | Sd c x, Sd d y =>
+    ev <- match_term ev (Ch c) (Ch d);
+    match_term ev x y
+  | Rv c x, Rv d y =>
+    ev <- match_term ev (Ch c) (Ch d);
+    match_term ev x y
+  | _, _ => None
+  end.
+
+Fixpoint match_trace (ev: sbst) (xs ys: list evt): option sbst :=
+  match xs, ys with
+  | [], [] => Some ev
+  | x :: xs, y :: ys =>
+    ev <- match_evt ev x y;
+    match_trace ev xs ys
+  | _, _ => None
+  end.
+
+Fixpoint match_list (ev: sbst) (xs ys: list alg): option sbst :=
+  match xs, ys with
+  | [], [] => Some ev
+  | x :: xs, y :: ys =>
+    ev <- match_term ev x y;
+    match_list ev xs ys
+  | _, _ => None
+end.
+
+(** ** Role Homomorphism
+
+    See if [x] matches one item in [ys]. *)
+
+Fixpoint match_one (ys: list alg) (ev: sbst) (x: alg): option sbst :=
+  match ys with
+  | [] => None
+  | y :: ys =>
+    match match_term ev x y with
+    | Some ev => Some ev
+    | None => match_one ys ev x
+    end
+  end.
+
+Definition match_uniqs (ev: sbst) (xs ys: list alg): option sbst :=
+  fold_m (match_one ys) ev xs.
+
+(** There exists a homomorphism from [x] to [y] iff the result is not
+    [None]. *)
+
+Definition homomorphism (x y: role): option sbst :=
+  ev <- match_trace [] (trace x) (trace y);
+  ev <- match_uniqs ev (uniqs x) (uniqs y);
+  ev <- match_list ev (inputs x) (inputs y);
+  match_list ev (outputs x) (outputs y).
