coq/Role.v
@@ -1,4 +1,4 @@
-Require Import List ListSet Bool Program Monad Alg.
+Require Import List ListSet Bool Program Monad Proc Alg.
 
 (** * Protocol Roles *)
 
@@ -22,19 +22,50 @@ Fixpoint has_no_dups (l: list alg): bool :=
   | x :: xs => not_in x xs && has_no_dups xs
   end.
 
-(** Is [p] a valid role? *)
+(** Is [r] a valid role? *)
 
-Definition valid_role (p: role): bool :=
-  match fold_m well_formed_event nil (trace p) with
+Definition valid_role (r: role): bool :=
+  match fold_m well_formed_event nil (trace r) with
   | None => false
   | Some decls =>
-    forallb (well_typed decls) (uniqs p) &&
-    forallb (flip orig (trace p)) (uniqs p) &&
-    forallb is_basic (uniqs p) &&
-    has_no_dups (uniqs p) &&
-    forallb (well_typed_with_chan decls) (inputs p) &&
-    forallb (fun x => is_chan x || is_basic x) (inputs p) &&
-    forallb (well_typed decls) (outputs p) &&
-    forallb (flip not_in (uniqs p)) (inputs p) &&
-    forallb (flip not_in (outputs p)) (inputs p)
+    forallb (well_typed decls) (uniqs r) &&
+    forallb (flip orig (trace r)) (uniqs r) &&
+    forallb is_basic (uniqs r) &&
+    has_no_dups (uniqs r) &&
+    forallb (well_typed_with_chan decls) (inputs r) &&
+    forallb (fun x => is_chan x || is_basic x) (inputs r) &&
+    forallb (well_typed decls) (outputs r) &&
+    forallb (flip not_in (uniqs r)) (inputs r) &&
+    forallb (flip not_in (outputs r)) (inputs r)
+  end.
+
+(** Executions are roles with exceptions.
+
+    - No variables of sort message are allowed in its trace.
+
+    - The order in which uniques occur in an execution is significant,
+      but it is not for a role.  In an execution, the order of the
+      uniques determines the order in which they are used to generate
+      nonces.  Within a role, uniques are just a set of basic
+      values. *)
+
+Definition is_not_mesg_decl (d: decl): bool :=
+  negb (type_eqb (snd d) Mesg).
+
+(** Is [r] a valid execution?  *)
+
+Definition valid_exec (r: role): bool :=
+  match fold_m well_formed_event nil (trace r) with
+  | None => false
+  | Some decls =>
+    forallb is_not_mesg_decl decls &&
+    forallb (well_typed decls) (uniqs r) &&
+    forallb (flip orig (trace r)) (uniqs r) &&
+    forallb is_basic (uniqs r) &&
+    has_no_dups (uniqs r) &&
+    forallb (well_typed_with_chan decls) (inputs r) &&
+    forallb (fun x => is_chan x || is_basic x) (inputs r) &&
+    forallb (well_typed decls) (outputs r) &&
+    forallb (flip not_in (uniqs r)) (inputs r) &&
+    forallb (flip not_in (outputs r)) (inputs r)
   end.
