coq/Sem.v
@@ -4,12 +4,11 @@
     role compiler. *)
 
 Require Import ListSet Bool Program Monad Proc Alg.
-Require Export Role.
+Require Export Role Match.
 Import List.ListNotations.
 Open Scope list_scope.
 Open Scope nat_scope.
 (** printing <- #←# *)
-(** printing ∘ %\ensuremath{\circ}% *)
 
 (** A runtime environment *)
 
@@ -111,7 +110,6 @@ Inductive stmt_sem: env -> list evt -> list alg ->
     lookup x ev = Some a ->
     lookup y ev = Some b ->
     a = b ->                    (* Sameness check *)
-    has_enc a = false ->        (* For probabilistic encryption *)
     stmt_sem ev tr us (Same x y) ev tr us.
 Hint Constructors stmt_sem : core.
 
@@ -172,121 +170,6 @@ Definition sem (p: proc) (ev: env) (e: role): Prop :=
   let ev_in := mk_env (ins p) (inputs e) in
   ins_inputs (ins p) (inputs e) /\
   stmt_list_sem ev_in (trace e) (uniqs e) (outputs e) (body p) ev [] [].
-
-(** ** Matching *)
-
-Definition extend_term (ev: env) (v: pvar) (x: alg): option env :=
-  match lookup v ev with
-  | None => Some ((v, x) :: ev)
-  | Some y =>
-    if alg_dec x y then
-      Some ev
-    else                        (* Term clash! *)
-      None
-  end.
-
-Definition match_skey (ev: env) (x y: skey): option env :=
-  match (x, y) with
-  | (Sv v, w) => extend_term ev v (Sk w)
-  | (Lt v w, Lt x y) =>
-    ev <- extend_term ev v (Nm x);
-    extend_term ev w (Nm y)
-  | _ => None
-  end.
-
-Definition match_akey (ev: env) (x y: akey): option env :=
-  match (x, y) with
-  | (Av v, w) => extend_term ev v (Ak w)
-  | (Pb v, Pb w) => extend_term ev v (Nm w)
-  | (Pb2 s v, Pb2 t w) =>
-    if string_dec s t then
-      extend_term ev v (Nm w)
-    else
-      None
-  | _ => None
-  end.
-
-Fixpoint match_term (ev: env) (x y: alg): option env :=
-  match (x, y) with
-  | (Tx v, Tx w) => extend_term ev v (Tx w)
-  | (Dt v, Dt w) => extend_term ev v (Dt w)
-  | (Nm v, Nm w) => extend_term ev v (Nm w)
-  | (Sk v, Sk w) => match_skey ev v w
-  | (Ak v, Ak w) => match_akey ev v w
-  | (Ak (Av v), Ik w) => extend_term ev v (Ik w)
-  | (Ik v, Ik w) => match_akey ev v w
-  | (Ik (Av v), Ak w) => extend_term ev v (Ik w)
-  | (Ch v, Ch w) => extend_term ev v (Ch w)
-  | (Mg v, w) => extend_term ev v w
-  | (Tg s, Tg t) =>
-    if string_dec s t then
-      Some ev
-    else
-      None
-  | (Pr v w, Pr x y) =>
-    ev <- match_term ev v x;
-    match_term ev w y
-  | (En v w, En x y) =>
-    ev <- match_term ev v x;
-    match_term ev w y
-  | (Hs v, Hs w) => match_term ev v w
-  | _ => None
-  end.
-
-Definition match_evt (ev: env) (x y: evt): option env :=
-  match (x, y) with
-  | (Sd c x, Sd d y) =>
-    ev <- match_term ev (Ch c) (Ch d);
-    match_term ev x y
-  | (Rv c x, Rv d y) =>
-    ev <- match_term ev (Ch c) (Ch d);
-    match_term ev x y
-  | _ => None
-  end.
-
-Fixpoint match_trace (ev: env) (xs ys: list evt): option env :=
-  match (xs, ys) with
-  | ([], []) => Some ev
-  | (x :: xs, y :: ys) =>
-    ev <- match_evt ev x y;
-    match_trace ev xs ys
-  | _ => None
-  end.
-
-Fixpoint match_list (ev: env) (xs ys: list alg): option env :=
-  match (xs, ys) with
-  | ([], []) => Some ev
-  | (x :: xs, y :: ys) =>
-    ev <- match_term ev x y;
-    match_list ev xs ys
-  | _ => None
-end.
-
-(** ** Role Homomorphism
-
-    See if [x] matches one item in [ys]. *)
-
-Fixpoint match_one (ys: list alg) (ev: env) (x: alg): option env :=
-  match ys with
-  | [] => None
-  | y :: ys =>
-    match match_term ev x y with
-    | Some ev => Some ev
-    | None => match_one ys ev x
-    end
-  end.
-
-Definition match_uniqs (ev: env) (xs ys: list alg): option env :=
-  fold_m (match_one ys) ev xs.
-
-(** There exists a homomorphism from [x] to [y] iff the result is not
-    [None]. *)
-
-Definition homomorphism (x y: role): option env :=
-  ev <- match_trace [] (trace x) (trace y);
-  ev <- match_uniqs ev (uniqs x) (uniqs y);
-  ev <- match_list ev (inputs x) (inputs y);
-  match_list ev (outputs x) (outputs y).
 
 (** ** Correct Input and Output *)
 
